Add conversion from Assignment to Clause; Change (weaken) Resolution rule definition

BSWLean/Treelike.lean
@@ -1,4 +1,6 @@
 import BSWLean.CNF
+import BSWLean.Substitutions
+import BSWLean.Conversion
 
 inductive TreeLikeResolution {vars} (φ : CNFFormula vars) : (c : Clause vars) → Type where
   | axiom_clause {c} (h_c_in_φ : c ∈ φ) : TreeLikeResolution φ c
@@ -9,8 +11,8 @@ inductive TreeLikeResolution {vars} (φ : CNFFormula vars) : (c : Clause vars) �
       (h_v_not_mem_c : v ∉ c.variables)
       (π₁ : TreeLikeResolution φ c₁)
       (π₂ : TreeLikeResolution φ c₂)
-      (h_resolve : (c ∪ { v.toLiteral h_v_mem_vars } = c₁) ∧
-                   (c ∪ { v.toNegLiteral h_v_mem_vars } = c₂))
+      (h_resolve : (c₁ ⊆ c ∪ { v.toLiteral h_v_mem_vars }) ∧
+                   (c₂ ⊆ c ∪ { v.toNegLiteral h_v_mem_vars }))
       : TreeLikeResolution φ c
 
 abbrev BotClause {vars} : Clause vars := ∅
@@ -44,7 +46,7 @@ lemma tree_like_proof_is_correct {vars} {φ : CNFFormula vars} (c : Clause vars)
     by_cases a v h_v_mem_vars
     case neg h =>
       obtain ⟨l₁, h_l₁_in_c₁, h_l₁_eval_a⟩ := ih₁
-      rw [←h_resolve.left] at h_l₁_in_c₁
+      apply Finset.mem_of_subset h_resolve.left at h_l₁_in_c₁
       use l₁
       simp only [h_l₁_eval_a, and_true]
       contrapose! h_l₁_in_c₁
@@ -59,7 +61,7 @@ lemma tree_like_proof_is_correct {vars} {φ : CNFFormula vars} (c : Clause vars)
       exact eq_false_of_ne_true h
     case pos h =>
       obtain ⟨l₂, h_l₂_in_c₂, h_l₂_eval_a⟩ := ih₂
-      rw [←h_resolve.right] at h_l₂_in_c₂
+      apply Finset.mem_of_subset h_resolve.right at h_l₂_in_c₂
       use l₂
       simp only [h_l₂_eval_a, and_true]
       contrapose! h_l₂_in_c₂
@@ -88,3 +90,187 @@ theorem tree_like_refutation_implies_unsat {vars} {φ : CNFFormula vars}
   simp only [ne_eq, Bool.not_eq_false] at h
   apply π a at h
   contradiction
+
+lemma CNFFormula.substitute_maintains_unsat {vars} (φ : CNFFormula vars)
+    (sub_vars : Variables) (h_subset : sub_vars ⊆ vars) (ρ' : Assignment sub_vars)
+    (h_unsat : Unsat φ)
+  : Unsat (φ.substitute sub_vars ρ') := by
+  constructor
+  intro ρ
+  by_contra!
+  simp only [ne_eq, Bool.not_eq_false] at this
+
+  let ρ_full : Assignment vars :=
+    fun v h_v_mem_vars =>
+      if h_v_mem : v ∈ sub_vars then
+        ρ' v h_v_mem
+      else
+        ρ v (by
+          refine Finset.mem_sdiff.mpr ?_
+          constructor
+          · exact h_v_mem_vars
+          · exact h_v_mem
+        )
+
+  have h_restrict_in : ρ_full.restrict (sub_vars) (by exact h_subset) = ρ' := by
+    unfold ρ_full
+    unfold Assignment.restrict
+    simp only
+    simp_all only [↓reduceDIte]
+
+  have h_restrict_out : ρ_full.restrict (vars \ sub_vars) (by exact Finset.sdiff_subset) = ρ := by
+    unfold ρ_full
+    unfold Assignment.restrict
+    simp only
+    have : ∀ v ∈ (vars \ sub_vars), v ∉ sub_vars := by
+      intro v h_v_mem_vars_sdiff
+      simp only [Finset.mem_sdiff] at h_v_mem_vars_sdiff
+      exact h_v_mem_vars_sdiff.2
+    simp_all only [↓reduceDIte]
+
+  have h_sub : ∀ c : Clause vars, c.eval ρ_full = true ↔
+    c.substitute sub_vars ρ' = none ∨
+     ∃ c' : Clause (vars \ sub_vars), c.substitute sub_vars ρ' = some c' ∧ c'.eval ρ = true := by
+    intro c
+    let (c_in, c_out) := c.split sub_vars
+    have h' : ρ_full.restrict (vars ∩ sub_vars) (by exact
+      Finset.inter_subset_left) = ρ'.restrict (vars ∩ sub_vars) (by
+        exact Finset.inter_subset_right) := by
+      have :vars ∩ sub_vars = sub_vars := by
+        exact Finset.inter_eq_right.mpr h_subset
+      rw [←h_restrict_in]
+      simp only [Assignment.double_restrict]
+
+    rw [Clause.split_correctness c sub_vars ρ_full
+    (by exact Finset.inter_subset_left) (by exact Finset.sdiff_subset)]
+
+    simp_all only [Bool.or_eq_true]
+    constructor
+
+    case mp =>
+      intro h
+      by_cases (c.split sub_vars).1.eval (ρ'.restrict (vars ∩ sub_vars) (by exact
+        Finset.inter_subset_right)) = true
+      case pos h_eval_c_in_true =>
+        left
+        rw [Clause.substitute_eq_none_iff_eval_subclause_true]
+        assumption
+      case neg h_eval_c_in_false =>
+        right
+        use (c.split sub_vars).2
+        constructor
+        · unfold Clause.substitute
+          simp_all only [Bool.false_eq_true, false_or, Bool.not_eq_true, ↓reduceIte]
+        · simp only [h_eval_c_in_false] at h
+          simp at h
+          assumption
+
+    case mpr =>
+      intro h
+      cases h
+      case inl h_c_subst_none =>
+        rw [Clause.substitute_eq_none_iff_eval_subclause_true] at h_c_subst_none
+        exact Or.symm (Or.inr h_c_subst_none)
+      case inr h_exists_c_out =>
+        obtain ⟨c_out, h_c_out_eval_ρ⟩ := h_exists_c_out
+        right
+        unfold Clause.substitute at h_c_out_eval_ρ
+        simp_all only [Option.ite_none_left_eq_some, Bool.not_eq_true, Option.some.injEq]
+
+
+  have h_eval_φ : φ.eval ρ_full = true := by
+    rw [CNFFormula.eval_eq_true_iff_all_satisfied_clauses]
+    intro c h_c_in_φ
+    rw [h_sub c]
+    by_cases h_ρ' : c.substitute sub_vars ρ' = none
+    case pos =>
+      left
+      assumption
+    case neg =>
+      right
+      let c_out := (c.substitute sub_vars ρ').get (by exact Option.isSome_iff_ne_none.mpr h_ρ')
+      use c_out
+      constructor
+      · simp_all only [Option.some_get, ρ_full, c_out]
+      · simp [c_out]
+        rw [CNFFormula.eval_eq_true_iff_all_satisfied_clauses] at this
+        unfold CNFFormula.substitute at this
+        simp_all only [Finset.mem_filterMap, Finset.mem_image, id_eq, exists_eq_right,
+          forall_exists_index, and_imp, ρ_full]
+        apply this
+        on_goal 2 => {
+          simp_all only [Option.some_get]
+          rfl
+        }
+        · simp_all only
+
+  have := h_unsat.h_unsat ρ_full
+  rw [h_eval_φ] at this
+  contradiction
+
+
+def TreeLikeResolution.size {vars} {φ : CNFFormula vars} :
+    ∀ {c : Clause vars}, TreeLikeResolution φ c → Nat
+  | _, .axiom_clause _ => 1
+  | _, .weakening _ _ π' => 1 + size π'
+  | _, .resolve _ _ _ _ _ π₁ π₂ _ => 1 + size π₁ + size π₂
+
+lemma TreeLikeResolution.unsubstitute {vars} {sub_vars} {φ : CNFFormula vars}
+    (h_subset : sub_vars ⊆ vars) (ρ : Assignment sub_vars) :
+    ∀ c' : Clause (vars \ sub_vars),
+    ∃ c : Clause vars, c' ∈ (c.substitute sub_vars ρ) ∧
+    ∀ π' : TreeLikeResolution (φ.substitute sub_vars ρ) c',
+    ∃ π : TreeLikeResolution φ c, π.size ≤ π'.size := by
+  intro c'
+  sorry
+
+theorem unsat_implies_tree_like_refutation {vars} {φ : CNFFormula vars}
+    (h_unsat : Unsat φ) : ∃ π : TreeLikeRefutation φ, π.size ≤ 2 * 2 ^ vars.card - 1 := by
+    induction vars using Finset.induction_on'
+    case empty =>
+      have h := h_unsat.h_unsat
+      have : BotClause ∈ φ := by
+        let a : Assignment ∅ := fun v h_v_mem_vars => by
+          exfalso
+          exact (List.mem_nil_iff v).mp h_v_mem_vars
+        specialize h a
+        rw [CNFFormula.eval_eq_false_iff_exists_falsified_clause] at h
+        obtain ⟨c, h_c_in_φ, h_c_eval_a_false⟩ := h
+        have h_c_eq_bot : c = BotClause := by
+          unfold BotClause
+          rw [@Finset.eq_empty_iff_forall_notMem]
+          intro l h_l_in_c
+          cases l
+          case pos v h_v_mem_vars =>
+            contradiction
+          case neg v h_v_mem_vars =>
+            contradiction
+        rw [←h_c_eq_bot]
+        exact h_c_in_φ
+      use TreeLikeResolution.axiom_clause this
+      simp only [Finset.card_empty, pow_zero]
+      unfold TreeLikeResolution.size
+      trivial
+
+    case insert v vars' h_v_in_vars h_subset h_v_not_in_vars' ih =>
+      let φ_true := φ.substitute {v} (fun _ => fun _ => True)
+      let φ_false := φ.substitute {v} (fun _ => fun _ => False)
+
+      have h_vars' : (insert v vars') \ {v} = vars' := by
+        rw [@Finset.sdiff_singleton_eq_erase]
+        rw [Finset.erase_insert h_v_not_in_vars']
+
+      have h_unsat_true : Unsat φ_true := by
+        refine CNFFormula.substitute_maintains_unsat φ {v} ?_ (fun x x_1 ↦ decide True) h_unsat
+        exact Finset.union_subset_left fun ⦃a⦄ a_1 ↦ a_1
+
+      have h_unsat_false : Unsat φ_false := by
+        refine CNFFormula.substitute_maintains_unsat φ {v} ?_ (fun x x_1 ↦ decide False) h_unsat
+        exact Finset.union_subset_left fun ⦃a⦄ a_1 ↦ a_1
+
+      rw [←h_vars'] at ih
+
+      obtain ⟨π_true, h_size_π_true⟩ := ih h_unsat_true
+      obtain ⟨π_false, h_size_π_false⟩ := ih h_unsat_false
+
+      sorry
