BSWLean.lean
@@ -1,3 +1,4 @@
 import BSWLean.CNF
+import BSWLean.Conversion
 import BSWLean.Treelike
 import BSWLean.Substitutions
