BSWLean/Conversion.lean
@@ -1,0 +1,142 @@
+import BSWLean.CNF
+
+def Assignment.negVariable {vars} (ρ : Assignment vars) (v : Variable) : Option (Literal vars) :=
+  if h_v_mem_vars : v ∈ vars then
+    if ρ v h_v_mem_vars then
+      some (Variable.toNegLiteral v h_v_mem_vars)
+    else
+      some (Variable.toLiteral v h_v_mem_vars)
+  else
+    none
+
+@[simp]
+lemma Assignment.negVariable_variable {vars} (ρ : Assignment vars)
+    (v : Variable) : ∀ y ∈ Assignment.negVariable ρ v, y.variable = v := by
+  intro y h
+  unfold Assignment.negVariable at h
+
+  aesop
+
+
+@[simp]
+lemma Assignment.negVariable_inj {vars} (ρ : Assignment vars) :
+  ∀ (x₁ x₂ : Variable), ∀ y ∈ Assignment.negVariable ρ x₁,
+    y ∈ Assignment.negVariable ρ x₂ → x₁ = x₂ := by
+  intros x₁ x₂ y h_y_in_mp_x1 h_y_in_mp_x2
+  unfold Assignment.negVariable at h_y_in_mp_x1 h_y_in_mp_x2
+  simp_all only [Option.mem_def, Option.dite_none_right_eq_some]
+  obtain ⟨h_x1_in_vars, h_y_eq_lit1⟩ := h_y_in_mp_x1
+  obtain ⟨h_x2_in_vars, h_y_eq_lit2⟩ := h_y_in_mp_x2
+  unfold Variable.toLiteral at h_y_eq_lit1 h_y_eq_lit2
+  unfold Variable.toNegLiteral at h_y_eq_lit1 h_y_eq_lit2
+
+  aesop
+
+lemma Assignment.negVariable_some_iff_variable_in_vars {vars} (ρ : Assignment vars) (v : Variable) :
+  (Assignment.negVariable ρ v).isSome ↔ v ∈ vars := by
+  unfold Assignment.negVariable
+
+  aesop
+
+def Assignment.toClause {vars} (ρ : Assignment vars) : Clause vars :=
+  vars.filterMap (Assignment.negVariable ρ) (Assignment.negVariable_inj ρ)
+
+lemma Assignment.in_toClause {vars} (ρ : Assignment vars) (l : Literal vars) :
+  l ∈ ρ.toClause ↔ (l.variable ∈ vars ∧ l.eval ρ = false) := by
+  unfold Assignment.toClause
+  simp only [Finset.mem_filterMap, Literal.variable_mem_vars, true_and]
+  constructor
+  case mpr =>
+    intro h_l_in_toClause
+    use l.variable
+    simp only [Literal.variable_mem_vars, true_and]
+    unfold Assignment.negVariable
+    unfold Literal.variable
+    unfold Literal.eval at h_l_in_toClause
+    simp_all only [Option.dite_none_right_eq_some]
+    split
+    next l v
+      h_v_mem_vars =>
+      simp_all only [Bool.false_eq_true, ↓reduceIte, Option.some.injEq, exists_true_left]
+      rfl
+    next l v
+      h_v_mem_vars =>
+      simp_all only [Bool.not_eq_eq_eq_not, Bool.not_false, ↓reduceIte, Option.some.injEq,
+                     exists_true_left]
+      rfl
+  case mp =>
+    intro h
+    obtain ⟨v, ⟨h_v_in_vars, h_l_eval_ρ_false⟩⟩ := h
+    unfold Assignment.negVariable at h_l_eval_ρ_false
+    unfold Literal.eval
+    unfold Variable.toLiteral Variable.toNegLiteral at h_l_eval_ρ_false
+
+    simp_all only [↓reduceDIte]
+    split
+    next l v_1 h_v_mem_vars =>
+      split at h_l_eval_ρ_false
+      next h => simp_all only [Option.some.injEq, reduceCtorEq]
+      next h => simp_all only [Bool.not_eq_true, Option.some.injEq, Literal.pos.injEq]
+    next l v_1 h_v_mem_vars =>
+      simp_all only [Bool.not_eq_eq_eq_not, Bool.not_false]
+      split at h_l_eval_ρ_false
+      next h => simp_all only [Option.some.injEq, Literal.neg.injEq]
+      next h => simp_all only [Bool.not_eq_true, Option.some.injEq, reduceCtorEq]
+
+
+lemma Assignment.toClause_eval {vars} (ρ : Assignment vars) :
+  ρ.toClause.eval ρ = false := by
+  unfold Assignment.toClause
+  rw [Clause.eval_eq_false_iff_all_falsified_literals]
+  intro l
+  unfold Assignment.negVariable
+  simp only [Finset.mem_filterMap, Option.dite_none_right_eq_some, and_exists_self,
+    forall_exists_index]
+  intro v h_v_mem_vars h_l_eq_lit
+  unfold Literal.eval
+  unfold Variable.toLiteral Variable.toNegLiteral at h_l_eq_lit
+
+  aesop
+
+lemma Assignment.toClause_variables {vars} (ρ : Assignment vars) :
+  ρ.toClause.variables = vars := by
+  unfold Clause.variables
+  ext v
+  constructor
+  case mpr =>
+    intro h_v_in_vars
+    simp only [Finset.mem_image]
+    let l := ρ.negVariable v
+    have h_l_some : l.isSome := by
+      rw [@negVariable_some_iff_variable_in_vars]
+      assumption
+    let l_some := l.get h_l_some
+    use l_some
+
+    constructor
+    · rw [@in_toClause]
+      simp_all only [Literal.variable_mem_vars, true_and, l_some, l]
+      unfold Assignment.negVariable
+      simp_all only [↓reduceDIte]
+      split
+      next h =>
+        simp_all only [Option.get_some]
+        unfold Variable.toNegLiteral
+        unfold Literal.eval
+        simp_all only [Bool.not_true]
+      next h =>
+        simp_all only [Option.get_some]
+        simp_all only [Bool.not_eq_true]
+        exact h
+
+    · unfold l_some l
+      rw [negVariable_variable ρ]
+      simp only [Option.mem_def, Option.some_get]
+
+  case mp =>
+    intro a
+    simp_all only [Finset.mem_image]
+    obtain ⟨w, h⟩ := a
+    obtain ⟨left, right⟩ := h
+    subst right
+    simp_all only [Literal.variable_mem_vars]
